\section{Complex Numbers}
\label{CmpNums}

We now move on to the study of the set of \sword{complex numbers}\index{numbers ! complex}\index{complex numbers}.  As you may recall, the complex numbers fill an algebraic gap left by the real numbers.  There is no real number $x$ with $x^2 = -1$, since for any real number $x^2 \geq 0$.  However, we could formally extract square roots and write $x = \pm \sqrt{-1}$.  We build the complex numbers by relabelling the quantity $\sqrt{-1}$ as $i$, the unfortunately misnamed \index{imaginary unit, $i$}\index{complex number ! imaginary unit, $i$}\sword{imaginary unit}.\footnote{Some Technical Mathematics textbooks label it `$j$'.  While it carries the adjective `imaginary', these numbers have essential real-world implications.  For example, every electronic device owes its existence to the study of `imaginary' numbers.}  The number $i$, while not a real number, is defined so that it plays along well with real numbers and acts very much like any other radical expression.  For instance, $3(2i) = 6i$, $7i-3i = 4i$, $(2-7i) + (3 + 4i) = 5-3i$, and so forth.  The key properties which distinguish $i$ from the real numbers are listed below.

\mnote{.7}{Historically, the lack of solutions to the equation $x^2=-1$ had nothing to do with the development of the complex numbers. Until the 19th century, equations such as $x^2=-1$ would have been considered in the context of the analytic geometry of Descartes. The lack of solutions simply indicated that the graph $y=x^2$ did not intersect the line $y=-1$. The more remarkable case was that of \textit{cubic} equations, of the form $x^3=ax+b$. In this case a \textbf{real} solution is \textit{guaranteed}, but there are cases where one needs \textbf{complex} numbers to find it! For details, see the excellent book \textit{Visual Complex Analysis}, by Tristan Needham.}

\medskip

\definition{idefn}{The imaginary unit}{
The imaginary unit $i$ satisfies the two following properties:

\begin{enumerate}

\item  $i^2 = -1$

\item  If $c$ is a real number with $c \geq 0$ then $\sqrt{-c} = i \sqrt{c}$

\end{enumerate}
}

\medskip

\mnote{.55}{Note the use of the indefinite article `a'.  Whatever beast is chosen to be $i$, $-i$ is the other square root of $-1$.}

Property 1 in Definition \ref{idefn} establishes that $i$ does act as a square root of $-1$, and property 2 establishes what we mean by the `principal square root' of a negative real number.  In property 2, it is important to remember the restriction on $c$.  For example, it is perfectly acceptable to say  $\sqrt{-4} = i \sqrt{4} = i(2) = 2i$. However, $\sqrt{-(-4)} \neq i \sqrt{-4}$, otherwise, we'd get\[ 2 = \sqrt{4} = \sqrt{-(-4)} = i \sqrt{-4} = i (2i) = 2i^2 = 2(-1) = -2,\] which is unacceptable. The moral of this story is that the general properties of radicals do not apply for even roots of negative quantities.  With Definition \ref{idefn} in place, we are now in position to define the \index{complex number ! definition of}\sword{complex numbers}.

\medskip

\definition{complexdefn}{Complex number}{
A \sword{complex number} is a number of the form $a+bi$, where $a$ and $b$ are real numbers and $i$ is the imaginary unit.  The set of complex numbers is denoted $\C$.
}

\medskip

Complex numbers include things you'd normally expect, like $3+2i$ and $\frac{2}{5} - i\sqrt{3}$.  However, don't forget that $a$ or $b$ could be zero, which means numbers like $3i$ and $6$ are also complex numbers.  In other words, don't forget that the complex numbers \textit{include} the real numbers, so $0$ and $\pi - \sqrt{21}$ are both considered complex numbers.   The arithmetic of complex numbers is as you would expect.  The only things you need to remember are the two properties in Definition \ref{idefn}.  The next example should help recall how these animals behave.

\mnote{.3}{To use the language  of Section \ref{SetsofNumbers}, $\R \subseteq \C$.}



\medskip

%\label{complexnumberarithmetic}

\example{complexzeroex1}{Arithmetic with complex numbers}{
Perform the indicated operations.


\begin{multicols}{3}
\begin{enumerate}

\item  $(1-2i) - (3+4i)$ \vphantom{$\dfrac{1-2i}{3-4i}$}
\item  $(1-2i)(3+4i)$ \vphantom{$\dfrac{1-2i}{3-4i}$}
\item  $\dfrac{1-2i}{3-4i}$

\setcounter{HW}{\value{enumi}}
\end{enumerate}
\end{multicols}

\begin{multicols}{3}
\begin{enumerate}
\setcounter{enumi}{\value{HW}}

\item  $\sqrt{-3} \sqrt{-12}$
\item  $\sqrt{(-3)(-12)}$
\item  $(x-[1+2i])(x-[1-2i])$

\setcounter{HW}{\value{enumi}}
\end{enumerate}
\end{multicols}
}
{
\begin{enumerate}

\item  As mentioned earlier, we treat expressions involving $i$ as we would any other radical. We distribute and combine like terms:\[ \begin{array}{rclr}

 (1-2i) - (3+4i) & = &  1-2i-3-4i & \text{Distribute} \\
                 & = &  -2 - 6i & \text{Gather like terms} \\
\end{array}\] Technically, we'd have to rewrite our answer  $-2-6i$ as $(-2) + (-6)i$ to be (in the strictest sense) `in the form $a+bi$'. That being said, even pedants have their limits, and we'll consider $-2-6i$ good enough.

\item  Using the Distributive Property (a.k.a. F.O.I.L.), we get \[ \begin{array}{rclr}

  (1-2i)(3+4i)  & = & (1)(3) + (1)(4i) - (2i)(3) - (2i)(4i) & \text{F.O.I.L.} \\
	              & = & 3+4i-6i-8i^2 & \\
								& = & 3 - 2i - 8(-1) & \text{$i^2=-1$} \\
								& = & 3 - 2i + 8 & \\
								& = & 11 - 2i & \\ \end{array}\]

\drawexampleline

\item  How in the world are we supposed to simplify $\frac{1-2i}{3-4i}$?  Well, we deal with the denominator $3-4i$ as we would any other denominator containing two terms, one of which is a square root: we and multiply both numerator and denominator by $3+4i$, the (complex) conjugate of $3 - 4i$.  Doing so produces\[\begin{array}{rclr}

 \dfrac{1-2i}{3-4i} & = & \dfrac{(1-2i)(3+4i)}{(3-4i)(3+4i)} & \text{Equivalent Fractions} \\[8pt]

                     & = &   \dfrac{3 + 4i - 6i - 8i^2}{9 - 16i^2} & \text{F.O.I.L.}\\[8pt]
										 & = & \dfrac{3 - 2i - 8(-1)}{9  - 16(-1)} & \text{$i^2 = -1$}\\[8pt]
						         & = &  \dfrac{11 - 2i}{25} & \\[8pt]
										  & = & \dfrac{11}{25} - \dfrac{2}{25} \, i & \\ \end{array}\]
										

\item  We use property 2 of Definition \ref{idefn} first, then apply the rules of radicals applicable to real numbers to get $\sqrt{-3} \sqrt{-12} = \left(i \sqrt{3}\right) \left(i \sqrt{12}\right) = i^2 \sqrt{3\cdot 12} = -\sqrt{36} = -6$.

\item  We adhere to the order of operations here and perform the multiplication before the radical to get  $\sqrt{(-3)(-12)} = \sqrt{36} = 6$. 

\item  We can brute force multiply using the distributive property and see that 
\begin{align*}
(x-[1+2i])(x-[1-2i]) & =  x^2 -x[1-2i]-x[1+2i]+[1-2i][1+2i]  \tag*{F.O.I.L.}\\								 & =  x^2-x+2ix-x-2ix+1-2i+2i-4i^2  \tag*{Distribute} \\								 & =  x^2-2x + 1-4(-1) \tag*{Gather like terms}\\										 & =  x^2 -2x +5  \tag*{$i^2=-1$}
\end{align*}
\end{enumerate}
}

\medskip

In the previous example, we used the idea of a `conjugate' to divide two complex numbers. (You may recall using conjugates to rationalize expressions involving square roots.)  More generally, the \index{complex number ! complex conjugate ! definition of}\index{conjugate ! complex conjugate ! definition of}\sword{complex conjugate} of a complex number $a+bi$ is the number $a-bi$.  The notation commonly used for complex conjugation is a `bar':  $\overline{a+bi} = a-bi$. For example, $\overline{3+2i} = 3-2i$ and $\overline{3-2i} = 3+2i$. To find $\overline{6}$, we note that $\overline{6} = \overline{6+0i}= 6 - 0i = 6$, so $\overline{6} = 6$. Similarly, $\overline{4i} = -4i$, since $\overline{4i} = \overline{0 + 4i} = 0 - 4i =  -4i$.  Note that $\overline{3+\sqrt{5}} = 3 + \sqrt{5}$, not $3 - \sqrt{5}$, since  $\overline{3+\sqrt{5}} = \overline{3+\sqrt{5} + 0i} = 3+\sqrt{5}  - 0i = 3+\sqrt{5}$. Here, the conjugation specified by the `bar' notation involves reversing the sign before $i = \sqrt{-1}$, not before  $\sqrt{5}$.  The properties of the conjugate are summarized in the following theorem.

\medskip

\theorem{conjugateprops}{Properties of the Complex Conjugate}{
\index{complex number ! conjugate ! properties of}\index{conjugate of a complex number ! properties of}
Let $z$ and $w$ be complex numbers. 

\begin{itemize}

\item  $\overline{\overline{z}} = z$

\item  $ \overline{z+w} = \overline{z} + \overline{w}$

\item  $ \overline{zw} = \overline{z} \, \overline{w}$

\item  $\overline{z^{n}} = \left(\overline{z}\right)^n$, for any natural number $n$

\item  $z$ is a real number if and only if $\overline{z} = z$.

\end{itemize}
}

\medskip

Essentially, Theorem \ref{conjugateprops} says that complex conjugation works well with addition, multiplication and powers.  The proofs of these properties can best be achieved by writing out $z = a+bi$ and $w = c+di$ for real numbers $a$, $b$, $c$ and $d$.   Next, we compute the left and right sides of each equation and verify that they are the same.  

\smallskip

The proof of the first property is a very quick exercise.  To prove the second property, we compare $\overline{z+w}$ with $\overline{z} + \overline{w}$.  We have $\overline{z} + \overline{w} = \overline{a+bi} + \overline{c+di}  = a-bi + c-di$.  To find $\overline{z+w}$, we first compute \[z+w = (a+bi) + (c+di) = (a+c)+(b+d)i\] so \[\overline{z+w} = \overline{(a+c)+(b+d)i} = (a+c) - (b+d)i = a - bi + c - di = \overline{z} + \overline{w}\]  As such, we have established  $\overline{z+w} = \overline{z}+\overline{w}$. The proof for multiplication works similarly.  The proof that the conjugate works well with powers can be viewed as a repeated application of the product rule, and is best proved using a technique called Mathematical Induction.  The last property is a characterization of real numbers.  If $z$ is real, then $z = a + 0i$, so $\overline{z} = a - 0i = a = z$.  On the other hand, if $z=\overline{z}$, then $a+bi = a - bi$ which means $b=-b$ so $b=0$.  Hence, $z = a +0i = a$ and is real.

\mnote{.85}{Proof by Mathematical Induction is usually taught in Math 2000.}

\mnote{.7}{We're assuming some prior familiarity on the part of the reader where quadratic equations are concerned. If you're a bit rusty when it comes to finding \textit{real} solutions to quadratic equations (and in particular, the quadratic formula), you may want to check out the review materials available on the ``Math Basics'' Moodle page.}

\medskip

We now consider the problem of solving quadratic equations. Consider  $x^2-2x+5 = 0$. The discriminant $b^2 - 4ac = -16$ is negative, so we know from the quadratic formula that there are no \textit{real} solutions, since the Quadratic Formula would involve the term $\sqrt{-16}$.  Complex numbers, however, are built just for such situations, so we can go ahead and apply the Quadratic Formula to get: \[ x = \dfrac{-(-2) \pm \sqrt{(-2)^2-4(1)(5)}}{2(1)} = \dfrac{2 \pm \sqrt{-16}}{2} = \dfrac{2 \pm 4i}{2} = 1 \pm 2i.\]  

\medskip

\example{complexsolnsreviewex}{Finding complex solutions}{
Find the complex solutions to the following equations.

\mnote{.52}{Remember, all real numbers are complex numbers, so `complex solutions' means both real and non-real answers.} 

\begin{multicols}{3}
\begin{enumerate}


\item  $\dfrac{2x}{x+1} = x+3$

\item $2t^4 = 9t^2 + 5$

\item  $z^3 + 1 = 0$

\end{enumerate}
\end{multicols}
}
{
\begin{enumerate}

%\enlargethispage{20pt}

\item  Clearing fractions yields a quadratic equation so we collect all terms on one side and apply the Quadratic Formula.\[ \begin{array}{rclr}


\dfrac{2x}{x+1} & = &  x+3 & \\[5pt]
2x & = & (x+3)(x+1) & \text{Multiply by $(x+1)$ to clear denominators} \\

2x & = & x^2 + x + 3x + 3 & \text{F.O.I.L.} \\

2x & = & x^2 + 4x + 3 & \text{Gather like terms} \\

0 & = & x^2 + 2x + 3 & \text{Subtract $2x$} \\

\end{array}\] From here, we apply the Quadratic Formula \[ \begin{array}{rclr}

x  & =  & \dfrac{-2 \pm \sqrt{2^2 - 4(1)(3)}}{2(1)}  & \text{Quadratic Formula}\\[8pt]
    & = &  \dfrac{-2 \pm \sqrt{-8}}{2} & \text{Simplify}\\[8pt]
		& =  & \dfrac{-2 \pm i \sqrt{8}}{2} & \text{Definition of $i$}\\[8pt]
		& =  & \dfrac{-2 \pm i 2\sqrt{2}}{2} & \text{Product Rule for Radicals}\\[8pt]
		& = & \dfrac{\cancel{2}(-1 \pm i\sqrt{2})}{\cancel{2}} & \text{Factor and reduce}\\[8pt]
		& = & -1 \pm i \sqrt{2} & \\
		\end{array} \]
		
We get two answers: $x = -1 + i\sqrt{2}$ and its conjugate $x = -1 - i\sqrt{2}$.  Checking both of these answers reviews all of the salient points about complex number arithmetic and is therefore strongly encouraged.

\item  Since we have three terms, and the exponent on one term (`$4$' on $t^4$) is exactly twice the exponent on the other (`$2$' on $t^2$), we have a Quadratic in Disguise.  We proceed accordingly.\[ \begin{array}{rclr}

2t^4 & = & 9t^2 + 5 & \\

2t^4 - 9t^2 - 5 & = & 0 & \text{Subtract $9t^2$ and $5$} \\
(2t^2 + 1)(t^2 - 5) & = & 0 & \text{Factor} \\
2t^2 + 1 = 0 & \text{or} & t^2 = 5 & \text{Zero Product Property} \\
\end{array}\]  From $2t^2 + 1 = 0$ we get $2t^2 = -1$, or $t^2 = -\frac{1}{2}$.  We extract square roots as follows: \[ t = \pm \sqrt{-\dfrac{1}{2}} = \pm i \sqrt{\dfrac{1}{2}} = \pm i \dfrac{\sqrt{1}}{\sqrt{2}} = \pm i \dfrac{1}{\sqrt{2}} = \pm \dfrac{i \sqrt{2}}{2},\]
where we have rationalized the denominator per convention.  From $t^2 = 5$, we get $t = \pm \sqrt{5}$. In total, we have four complex solutions - two real: $t = \pm \sqrt{5}$ and two non-real: $t = \pm \frac{i \sqrt{2}}{2}$.

\item To find  the \textit{real} solutions to  $z^3 + 1 = 0$, we can subtract the $1$ from both sides and extract cube roots: $z^3 = -1$, so $z  = \sqrt[3]{-1} = -1$.  It turns out there are two more non-real complex number solutions to this equation.  To get at these, we factor:\[ \begin{array}{rclr}

z ^ 3 + 1 & = & 0 & \\
(z + 1)(z^2 - z + 1) & = & 0 & \text{Factor (Sum of Two Cubes)} \\
z + 1 = 0 & \text{or} & z^2 - z + 1 = 0 & \\
\end{array} \] From $z+1 = 0$, we get our real solution $z = -1$.  From $z^2 -z + 1 = 0$, we apply the Quadratic Formula to get: \[z = \dfrac{-(-1) \pm \sqrt{(-1)^2 - 4(1)(1)}}{2(1)} = \dfrac{1 \pm \sqrt{-3}}{2} = \dfrac{1 \pm i\sqrt{3}}{2} \]
Thus we get \textit{three} solutions to $z^3 + 1 = 0$ - one real: $z = -1$ and two non-real: $z =  \frac{1 \pm i\sqrt{3}}{2}$.  As always, the reader is encouraged to test their algebraic mettle and check these solutions. 
		
\end{enumerate}
}

\medskip

It is no coincidence that the non-real solutions to the equations in Example \ref{complexsolnsreviewex} appear in  complex conjugate pairs. Any time we use the Quadratic Formula to solve an equation with \underline{real} coefficients, the answers will form a  complex conjugate pair owing to the $\pm$ in the Quadratic Formula.  This is stated formally in the following theorem.

\smallskip

\theorem{discriminanttheoremcomplexversion}{Discriminant Theorem}{
Given a Quadratic Equation $AX^2 + BX + C = 0$, where $A$, $B$ and $C$ are real numbers, let $D = B^2 - 4AC$ be the discriminant.

\begin{itemize}

\item  If $D > 0$, there are two distinct real number solutions to the equation. 

\item  If $D = 0$, there is one (repeated) real number solution.  

\textbf{Note:}  `Repeated' here comes from the fact that `both' solutions $\frac{-B \pm 0}{2A}$ reduce to $-\frac{B}{2A}$.

\item  If $D < 0$, there are two non-real solutions which form a complex conjugate pair.

\end{itemize}
}

\medskip

Theorem \ref{discriminanttheoremcomplexversion} tells us that if ever we obtain non-real zeros to a quadratic function with \underline{real} coefficients, the zeros  will be a complex conjugate pair. (Do you see why?)  Next, we note that in Example \ref{complexzeroex1}, part 6, we found $(x-[1+2i])(x-[1-2i])=x^2-2x+5$.  This demonstrates that the factor theorem holds even for non-real zeros, i.e,  $x=1+2i$ is a zero of $f$, and, sure enough, $(x-[1+2i])$ is a factor of $f(x)$.  It turns out that polynomial division works the same way for all complex numbers, real and non-real alike, so the Factor and Remainder Theorems hold as well.  But how do we know if a general polynomial has any complex zeros at all?  We have many examples of polynomials with no real zeros.  Can there be polynomials with no zeros whatsoever?  The answer to that last question is ``No.'' and the theorem which provides that answer is \index{Fundamental Theorem of Algebra} The Fundamental Theorem of Algebra.

\medskip

\theorem{ftoa}{The Fundamental Theorem of Algebra}{\index{Fundamental Theorem of Algebra} \index{theorem ! Fundamental Theorem of Algebra}  Suppose $f$ is a polynomial function with complex number coefficients of degree $n \geq 1$, then $f$ has at least one complex zero.
}

\medskip

The Fundamental Theorem of Algebra is an example of an `existence' theorem in Mathematics.  It  guarantees the existence of at least one zero, but gives us no algorithm to use in finding it.  The authors are fully aware that the full impact and profound nature of the Fundamental Theorem of Algebra  is lost on most students, and that's fine.  It took mathematicians literally hundreds of years to prove the theorem in its full generality, and some of that history is recorded \href{http://en.wikipedia.org/wiki/Fundamental_theorem_of_algebra}{\underline{in this Wikipedia article}}.  Note that the Fundamental Theorem of Algebra  applies to not only polynomial functions with real coefficients, but to those with complex number coefficients as well.  

\mnote{.25}{The Fundamental Theorem of Algebra has since been proved many times, using many different methods, by many mathematicians. There are probably very few, if any, results in mathematics with the variety of proofs this result has. Unfortunately, none of the proofs can be understood within the realm of this text, but if the reader is sufficiently interested, a collection of proofs can be found at \href{http://www.cut-the-knot.org/fta/analytic.shtml}{\underline{this website}}.}


\smallskip

Suppose  $f$ is a polynomial of degree $n \geq 1$.  The Fundamental Theorem of Algebra guarantees us at least one complex zero, $z_{\mbox{\tiny $1$}}$, and as such, the Factor Theorem guarantees that $f(x)$ factors as $f(x) = \left(x - z_{\mbox{\tiny $1$}}\right) q_{\mbox{\tiny $1$}}(x)$ for a polynomial function $q_{\mbox{\tiny $1$}}$,  of degree exactly $n-1$.  If $n-1 \geq 1$, then the Fundamental Theorem of Algebra guarantees a complex zero of $q_{\mbox{\tiny $1$}}$ as well, say $z_{\mbox{\tiny $2$}}$, so then the Factor Theorem gives us $q_{\mbox{\tiny $1$}}(x) = \left(x - z_{\mbox{\tiny $2$}}\right) q_{\mbox{\tiny $2$}}(x)$, and hence $f(x) = \left(x - z_{\mbox{\tiny $1$}}\right) \left(x - z_{\mbox{\tiny $2$}}\right) q_{\mbox{\tiny $2$}}(x)$.  We can continue this process exactly $n$ times, at which point our quotient polynomial $q_{\mbox{\tiny $n$}}$ has degree $0$ so it's a constant.  This argument gives us the following factorization theorem.

\smallskip

\theorem{complexfactorization}{Complex Factorization Theorem}{ Suppose $f$ is a polynomial function with complex number coefficients.  If the degree of $f$ is $n$ and $n \geq 1$, then  $f$ has exactly $n$ complex zeros, counting multiplicity.  If $z_{\mbox{\tiny $1$}}$, $z_{\mbox{\tiny $2$}}$, \ldots, $z_{\mbox{\tiny $k$}}$ are the distinct zeros of $f$, with multiplicities $m_{\mbox{\tiny $1$}}$, $m_{\mbox{\tiny $2$}}$, \ldots, $m_{\mbox{\tiny $k$}}$, respectively, then $f(x) = a\left(x - z_{\mbox{\tiny $1$}}  \right)^{m_{\mbox{\tiny $1$}}}\left(x - z_{\mbox{\tiny $2$}}  \right)^{m_{\mbox{\tiny $2$}}} \cdots \left(x - z_{\mbox{\tiny $k$}}  \right)^{m_{\mbox{\tiny $k$}}}$. \index{Complex Factorization Theorem}\index{factorization ! over the complex numbers}
}


\printexercises{exercises/00_04_exercises}